minuska/theories/examples.v
@@ -14,6 +14,22 @@ From Minuska Require Import
     frontend
 .
 
+Fixpoint interp_loop
+    {Σ : StaticModel}
+    (interp : GroundTerm -> option GroundTerm)
+    (fuel : nat)
+    (g : GroundTerm)
+    : (nat*GroundTerm)
+:=
+match fuel with
+| 0 => (0,g)
+| S fuel' =>
+    match interp g with
+    | None => (fuel', g)
+    | Some g' => interp_loop interp fuel' g'
+    end
+end
+.
 
 Module example_1.
 
@@ -26,11 +42,11 @@ Module example_1.
     
     Definition X : variable := "X".
 
-    Definition cfg {_r : Resolver} := (apply_symbol "cfg").
-    Arguments cfg {_r} _%rs.
+    Definition cfg {_br : BasicResolver} := (apply_symbol "cfg").
+    Arguments cfg {_br} _%rs.
 
-    Definition s {_r : Resolver} := (apply_symbol "s").
-    Arguments s {_r} _%rs.
+    Definition s {_br : BasicResolver} := (apply_symbol "s").
+    Arguments s {_br} _%rs.
 
     Definition Decls : list Declaration := [
         rule ["my_rule"]:
@@ -49,11 +65,15 @@ Module example_1.
     Fixpoint interp_loop
         (fuel : nat)
         (g : GroundTerm)
-        : option GroundTerm
+        : (nat*GroundTerm)
     :=
     match fuel with
-    | 0 => Some g
-    | S fuel' => g' ← interp g; interp_loop fuel' g'
+    | 0 => (0,g)
+    | S fuel' =>
+        match interp g with
+        | None => (fuel', g)
+        | Some g' => interp_loop fuel' g'
+        end
     end
     .
 
@@ -119,9 +139,8 @@ Module example_1.
 
     Definition interp_loop_number fuel := 
         fun n =>
-        let og' := ((interp_loop fuel) ∘ my_number) n in
-        g' ← og';
-        my_number_inv g'
+        let fg' := ((interp_loop fuel) ∘ my_number) n in
+        my_number_inv fg'.2
     .
 
 End example_1.
@@ -138,14 +157,14 @@ Module two_counters.
     Definition M : variable := "M".
     Definition N : variable := "N".
     
-    Definition cfg {_r : Resolver} := (apply_symbol "cfg").
-    Arguments cfg {_r} _%rs.
+    Definition cfg {_br : BasicResolver} := (apply_symbol "cfg").
+    Arguments cfg {_br} _%rs.
 
-    Definition state {_r : Resolver} := (apply_symbol "state").
-    Arguments state {_r} _%rs.
+    Definition state {_br : BasicResolver} := (apply_symbol "state").
+    Arguments state {_br} _%rs.
 
-    Definition s {_r : Resolver} := (apply_symbol "s").
-    Arguments s {_r} _%rs.
+    Definition s {_br : BasicResolver} := (apply_symbol "s").
+    Arguments s {_br} _%rs.
 
     Definition Γ : FlattenedRewritingTheory :=
     Eval vm_compute in (to_theory (process_declarations ([
@@ -157,17 +176,6 @@ Module two_counters.
 
     Definition interp :=
         naive_interpreter Γ
-    .
-
-    Fixpoint interp_loop
-        (fuel : nat)
-        (g : GroundTerm)
-        : option GroundTerm
-    :=
-    match fuel with
-    | 0 => Some g
-    | S fuel' => g' ← interp g; interp_loop fuel' g'
-    end
     .
 
     Definition pair_to_state (mn : nat*nat) : GroundTerm :=
@@ -214,9 +222,8 @@ Module two_counters.
 
     Definition interp_loop_number fuel := 
         fun (m n : nat) =>
-        let og' := ((interp_loop fuel) ∘ pair_to_state) (m,n) in
-        g' ← og';
-        state_to_pair g'
+        let fg' := ((interp_loop interp fuel) ∘ pair_to_state) (m,n) in
+        state_to_pair fg'.2
     .
 
 End two_counters.
@@ -233,49 +240,102 @@ Module arith.
     Definition Y : variable := "Y".
     Definition REST_SEQ : variable := "$REST_SEQ".
     
-    Definition cseq {_r : Resolver} := (apply_symbol "cseq").
-    Arguments cseq {_r} _%rs.
+    Definition cseq {_br : BasicResolver} := (apply_symbol "cseq").
+    Arguments cseq {_br} _%rs.
 
-    Definition emptyCseq {_r : Resolver} := (apply_symbol "emptyCseq").
-    Arguments emptyCseq {_r} _%rs.
+    Definition emptyCseq {_br : BasicResolver} := (apply_symbol "emptyCseq").
+    Arguments emptyCseq {_br} _%rs.
 
-    Definition plus {_r : Resolver} := (apply_symbol "plus").
-    Arguments plus {_r} _%rs.
+    Definition plus {_br : BasicResolver} := (apply_symbol "plus").
+    Arguments plus {_br} _%rs.
 
-    Definition cfg {_r : Resolver} := (apply_symbol "cfg").
-    Arguments cfg {_r} _%rs.
+    Definition cfg {_br : BasicResolver} := (apply_symbol "cfg").
+    Arguments cfg {_br} _%rs.
 
-    Definition state {_r : Resolver} := (apply_symbol "state").
-    Arguments state {_r} _%rs.
+    Definition state {_br : BasicResolver} := (apply_symbol "state").
+    Arguments state {_br} _%rs.
 
-    Definition s {_r : Resolver} := (apply_symbol "s").
-    Arguments s {_r} _%rs.
+    Definition s {_br : BasicResolver} := (apply_symbol "s").
+    Arguments s {_br} _%rs.
+
+    Definition freezer {_br : BasicResolver} (sym : symbol) (position : nat)
+    :=
+        (apply_symbol ("freezer_" +:+ sym +:+ "_" +:+ (pretty position)))
+    .
+    Arguments freezer {_br} _%rs.
+
 
     Declare Scope LangArithScope.
     Delimit Scope LangArithScope with larith.
 
     Notation "x '+' y" := (plus [ x, y ]).
-    
+
+    Definition isResult (x : Expression) : Expression :=
+        (isNat x)
+    .
+
     Definition Decls : list Declaration := [
         rule ["plus-nat-nat"]:
              cfg [ cseq [ ($X + $Y), $REST_SEQ ] ]
-          ~> (cfg [ (cseq [ (($X +Nat $Y) +Nat $Y) , $REST_SEQ ])%rs ])%rs
+          ~> (cfg [ (cseq [ ($X +Nat $Y) , $REST_SEQ ])%rs ])%rs
              where (
-                (isNat $X)
+                (isNat ($X))
                 &&
-                (isNat $Y)
+                (isNat ($Y))
              )
-        (*;
-        (* TODO *)
-        rule ["plus-heat-any"]:
-             top [< cseq [< plus [< $X, $Y >], $REST_SEQ >] >]
-          => top [< cseq [< ($X +Nat $Y) , $REST_SEQ >] >]
-        *)   
-
+        ;
+        rule ["plus-heat-1"]:
+             cfg [ cseq [ plus [ $X, $Y ], $REST_SEQ ]]
+          ~> cfg [ cseq [$X, cseq [ (freezer "plus" 0) [$Y] , $REST_SEQ ]]]
+             where ( ~~ (isResult ($X)) )
+        ;
+        rule ["plus-cool-1"]: 
+             cfg [ cseq [$X, cseq [ (freezer "plus" 0) [$Y] , $REST_SEQ ]]]
+          ~> cfg [ cseq [ plus [ $X, $Y ], $REST_SEQ ]]
+             where ((isResult ($X)) )
+        ;
+        rule ["plus-heat-2"]:
+             cfg [ cseq [ plus [ $X, $Y ], $REST_SEQ ]]
+          ~> cfg [ cseq [$Y, cseq [ (freezer "plus" 1) [$X] , $REST_SEQ ]]]
+             where ( isResult ($X) && ~~ (isResult ($Y)) )
+        ;
+        rule ["plus-cool-2"]: 
+             cfg [ cseq [$Y, cseq [ (freezer "plus" 1) [$X] , $REST_SEQ ]]]
+          ~> cfg [ cseq [ plus [ $X, $Y ], $REST_SEQ ]]
+             where ((isResult ($Y)) )
     ].
 
     Definition Γ : FlattenedRewritingTheory := Eval vm_compute in 
     (to_theory (process_declarations (Decls))).
+
+    Definition initial1 (x y : nat) :=
+        (ground (cfg [ cseq [ ((@aoo_operand symbol _ (bv_nat x)) + (@aoo_operand symbol _ (bv_nat y))), emptyCseq [] ] ]))
+    .
+
+    Definition initial (x: nat) (ly : list nat) :=
+        (ground (
+            cfg [
+                cseq ([ 
+                    (foldr 
+                        (fun a (b : AppliedOperatorOr' symbol builtin_value) =>
+                            plus [((bv_nat a)) , b]
+                        )
+                        (@aoo_operand symbol builtin_value (bv_nat x))
+                        ly
+                    ),
+                    emptyCseq []
+                    ])%rs
+                ]
+            )
+        )
+    .
+
+    Definition interp_list (fuel : nat) (x : nat) (ly : list nat)
+    :=
+        interp_loop (naive_interpreter Γ) fuel (initial x ly)
+    .
+
+    Eval vm_compute in (interp_list 20 1 [20;30;40]).
 
 End arith.
 
